# Lesson 5 - 4/9/2023

* F = ma
* a = dv/dt
* Fdt = m dv = d(mv)
* impetus = change in momentum

* Center of mass --> is a weighted average

* mv * a -> mv dv /dt -> d(1/2mv^2)/dt -> d(KE)/dt
```
1*6 + 2*3 = 12 --> v = 4
18 + 9 = 27, 24 -> 3J
```

* 1/2kx^2 = 1/2mv^2
* v = sqrt(k/m)x
* mv = m sqrt(k/m) x = sqrt(mk) x


* m1v1 + m2v2 = 28
* 1/2m1v1^2 + 1/2m2v2^2 = 104

```
v1 + 4v2=28
1/2v1^2 + 2v2^2 = 104

v1 = 28-4v2
0.5 (28-4v)^2 + 2v^2 = 104
0.5(28^2 - 2*28*4v + 16v^2) + 2v^2 = 104
10v^2 -112v + 288 = 0
v^2 - 11.2 + 28.8 = 0
```

* 0.1, 4 -> x, Vx=4, Vy = 0
* 0.1, 2 at 43degree --> Vx = 2cos(43)=1.46;  Vy = 2 * sin(43) = 1.36
* m=0.4, m1vy1=m2vy2, 0.1 * 1.36 = 0.4 vy2, vy2 = 0.34
* ....              , 0.1 * 4 = 0.1 * 1.46 + 0.4 vx2, vx2 = 0.635
* v = sqrt(0.34*0.34+0.64*0.64) = 0.72, sin(t) = 0.52, theta = -32degree  
